feat: introduce `has_usage` to improve bytes invariant

src/core/DY.Core.Bytes.Type.fst
@@ -4,6 +4,56 @@ module DY.Core.Bytes.Type
 /// It is separated from functions and predicates on bytes
 /// in order to avoid dependency cycles.
 
+/// The bytes term.
+/// It is similar to the one you would find in other symbolic analysis tools.
+/// One notable difference is that this one only contains "constructors" (e.g. encryption)
+/// and omit "destructors" (e.g. decryption).
+/// This is because while other symbolic analysis tools
+/// often reason on equality modulo some rewriting rules
+/// (such as `dec(k, enc(k, msg)) == msg`).
+/// Reasoning on equality "modulo something" in F* is cumbersome.
+/// Instead, the destructors (e.g. decryption) will inspect the bytes
+/// and return the data you would obtain via the reduction rule
+/// (e.g. the plaintext if the bytes is an encryption with the correct key).
+/// This allows us to reason with F*'s logical equality (`==`).
+
+type bytes =
+  // Public values (strings, numbers, ...)
+  | Literal: FStar.Seq.seq FStar.UInt8.t -> bytes
+  // Randomly generated numbers. `time` is used to ensure two random numbers are distinct.
+  | Rand: len:nat{len <> 0} -> time:nat -> bytes
+
+  // Concatenation
+  | Concat: left:bytes -> right:bytes -> bytes
+
+  // Authenticated (private key) Encryption with Additional Data
+  | AeadEnc: key:bytes -> nonce:bytes -> msg:bytes -> ad:bytes -> bytes
+
+  // Public key encryption
+  | Pk: sk:bytes -> bytes
+  | PkEnc: pk:bytes -> nonce:bytes -> msg:bytes -> bytes
+
+  // Signature
+  | Vk: sk:bytes -> bytes
+  | Sign: sk:bytes -> nonce:bytes -> msg:bytes -> bytes
+
+  // Hash
+  | Hash: msg:bytes -> bytes
+
+  // Diffie-Hellman
+  | DhPub: sk:bytes -> bytes
+  | Dh: sk:bytes -> pk:bytes -> bytes
+
+  // Key Derivation Function
+  | KdfExtract: salt:bytes -> ikm:bytes -> bytes
+  | KdfExpand: prk:bytes -> info:bytes -> len:nat{len <> 0} -> bytes
+
+  // Key Encapsulation Mechanism
+  | KemPub: sk:bytes -> bytes
+  | KemEncap: pk:bytes -> ss:bytes -> bytes
+  | KemSecretShared: ss:bytes -> bytes
+  // ...
+
 /// Usages depict how a given bytestring will be cryptographically used.
 ///
 /// First, it will say whether a bytestring is e.g. a signature key or a symetric encryption key.
@@ -37,84 +87,17 @@ type usage =
   | PkNonce: usage
   | AeadKey: tag:string -> data:bytes -> usage
   | DhKey: tag:string -> data:bytes -> usage
-  | KdfExtractSaltKey: tag:string -> data:bytes -> usage
-  | KdfExtractIkmKey: tag:string -> data:bytes -> usage
   | KdfExpandKey: tag:string -> data:bytes -> usage
   | KemKey: usg:usage -> usage
   | KemNonce: usg:usage -> usage
 
-/// The bytes term.
-/// It is similar to the one you would find in other symbolic analysis tools.
-/// One notable difference is that this one only contains "constructors" (e.g. encryption)
-/// and omit "destructors" (e.g. decryption).
-/// This is because while other symbolic analysis tools
-/// often reason on equality modulo some rewriting rules
-/// (such as `dec(k, enc(k, msg)) == msg`).
-/// Reasoning on equality "modulo something" in F* is cumbersome.
-/// Instead, the destructors (e.g. decryption) will inspect the bytes
-/// and return the data you would obtain via the reduction rule
-/// (e.g. the plaintext if the bytes is an encryption with the correct key).
-/// This allows us to reason with F*'s logical equality (`==`).
-
-and bytes =
-  // Public values (strings, numbers, ...)
-  | Literal: FStar.Seq.seq FStar.UInt8.t -> bytes
-  // Randomly generated numbers. `time` is used to ensure two random numbers are distinct.
-  | Rand: usage:usage -> len:nat{len <> 0} -> time:nat -> bytes
-
-  // Concatenation
-  | Concat: left:bytes -> right:bytes -> bytes
-
-  // Authenticated (private key) Encryption with Additional Data
-  | AeadEnc: key:bytes -> nonce:bytes -> msg:bytes -> ad:bytes -> bytes
-
-  // Public key encryption
-  | Pk: sk:bytes -> bytes
-  | PkEnc: pk:bytes -> nonce:bytes -> msg:bytes -> bytes
-
-  // Signature
-  | Vk: sk:bytes -> bytes
-  | Sign: sk:bytes -> nonce:bytes -> msg:bytes -> bytes
-
-  // Hash
-  | Hash: msg:bytes -> bytes
-
-  // Diffie-Hellman
-  | DhPub: sk:bytes -> bytes
-  | Dh: sk:bytes -> pk:bytes -> bytes
-
-  // Key Derivation Function
-  | KdfExtract: salt:bytes -> ikm:bytes -> bytes
-  | KdfExpand: prk:bytes -> info:bytes -> len:nat{len <> 0} -> bytes
-
-  // Key Encapsulation Mechanism
-  | KemPub: sk:bytes -> bytes
-  | KemEncap: pk:bytes -> ss:bytes -> bytes
-  | KemSecretShared: ss:bytes -> bytes
-  // ...
-
 open DY.Core.Internal.Ord
 
-val encode_usage: usage -> list int
 val encode_bytes: bytes -> list int
-let rec encode_usage usg =
-  match usg with
-  | NoUsage -> 0::[]
-  | SigKey tag data -> 1::(encode_list [encode tag; encode_bytes data])
-  | SigNonce -> 2::[]
-  | PkKey tag data -> 3::(encode_list [encode tag; encode_bytes data])
-  | PkNonce -> 4::[]
-  | AeadKey tag data -> 5::(encode_list [encode tag; encode_bytes data])
-  | DhKey tag data -> 6::(encode_list [encode tag; encode_bytes data])
-  | KdfExtractSaltKey tag data -> 7::(encode_list [encode tag; encode_bytes data])
-  | KdfExtractIkmKey tag data -> 8::(encode_list [encode tag; encode_bytes data])
-  | KdfExpandKey tag data -> 9::(encode_list [encode tag; encode_bytes data])
-  | KemKey usg -> 10::(encode_list [encode_usage usg])
-  | KemNonce usg -> 11::(encode_list [encode_usage usg])
-and encode_bytes b =
+let rec encode_bytes b =
   match b with
   | Literal l -> 0::(encode_list [encode l])
-  | Rand usg len time -> 1::(encode_list [encode_usage usg; encode (len <: nat); encode time])
+  | Rand len time -> 1::(encode_list [encode (len <: nat); encode time])
   | Concat left right -> 2::(encode_list [encode_bytes left; encode_bytes right])
   | AeadEnc key nonce msg ad -> 3::(encode_list [encode_bytes key; encode_bytes nonce; encode_bytes msg; encode_bytes ad])
   | Pk sk -> 4::(encode_list [encode_bytes sk])
@@ -130,41 +113,18 @@ and encode_bytes b =
   | KemEncap pk ss -> 14::(encode_list [encode_bytes pk; encode_bytes ss])
   | KemSecretShared ss -> 15::(encode_list [encode_bytes ss])
 
-// --warn_error is a workaround for FStar/FStarLang#3220
-#push-options "--z3rlimit 25 --fuel 3 --ifuel 3 --warn_error +290"
-val encode_usage_inj: usg1:usage -> usg2:usage -> Lemma (requires encode_usage usg1 == encode_usage usg2) (ensures usg1 == usg2)
+#push-options "--z3rlimit 25 --fuel 3 --ifuel 3"
 val encode_bytes_inj: b1:bytes -> b2:bytes -> Lemma (requires encode_bytes b1 == encode_bytes b2) (ensures b1 == b2)
-let rec encode_usage_inj usg1 usg2 =
-  encode_inj_forall (list (list int)) ();
-  match usg1, usg2 with
-  | SigNonce, SigNonce
-  | PkNonce, PkNonce
-  | NoUsage, NoUsage -> ()
-  | SigKey tag1 data1, SigKey tag2 data2
-  | PkKey tag1 data1, PkKey tag2 data2
-  | AeadKey tag1 data1, AeadKey tag2 data2
-  | DhKey tag1 data1, DhKey tag2 data2
-  | KdfExtractSaltKey tag1 data1, KdfExtractSaltKey tag2 data2
-  | KdfExtractIkmKey tag1 data1, KdfExtractIkmKey tag2 data2
-  | KdfExpandKey tag1 data1, KdfExpandKey tag2 data2 -> (
-    encode_inj tag1 tag2;
-    encode_bytes_inj data1 data2
-  )
-  | KemKey usg1, KemKey usg2
-  | KemNonce usg1, KemNonce usg2 ->
-    encode_usage_inj usg1 usg2
-
-and encode_bytes_inj b1 b2 =
+let rec encode_bytes_inj b1 b2 =
   encode_inj_forall (list (list int)) ();
   match b1, b2 with
   | Literal x1, Literal x2 ->
     encode_list_inj [encode x1] [encode x2];
     encode_inj x1 x2
-  | Rand x1 x2 x3, Rand y1 y2 y3 ->
-    encode_list_inj [encode_usage x1; encode (x2 <: nat); encode x3] [encode_usage y1; encode (y2 <: nat); encode y3];
-    encode_usage_inj x1 y1;
-    encode_inj x2 y2;
-    encode_inj x3 y3
+  | Rand x1 x2, Rand y1 y2 ->
+    encode_list_inj [encode (x1 <: nat); encode x2] [encode (y1 <: nat); encode y2];
+    encode_inj x1 y1;
+    encode_inj x2 y2
   | Pk x1, Pk y1
   | Vk x1, Vk y1
   | Hash x1, Hash y1
@@ -191,11 +151,6 @@ and encode_bytes_inj b1 b2 =
     encode_bytes_inj x4 y4
   | _, _ -> assert(False)
 #pop-options
-
-instance integer_encodable_usage: integer_encodable usage = {
-  encode = encode_usage;
-  encode_inj = encode_usage_inj;
-}
 
 instance integer_encodable_bytes: integer_encodable bytes = {
   encode = encode_bytes;
